\chapter{Numbers of Various Sorts}
\begin{pr} \label{2.1}% 2.1
  Prove the following formula by induction.
  \begin{enumerate}[label=(\roman*)]
    \item \label{2.1:i}
    $1^2+\dots+n^2=\dfrac{n(n+1)(2n+1)}{6}$.
    \item $1^3+\dots+n^3=(1+\dots+n)^2$.
  \end{enumerate}
\end{pr}

\begin{solution} % s2.1
  \begin{enumerate}[label=(\roman*)]
    \item If $n=1$, the equation holds. Suppose the
    equation holds for $n=k$, then for $n=k+1$,
    \begin{IEEEeqnarray*}{lC}
      & 1^2+\dots+k^2+(k+1)^2 \\
    = & \frac{k(k+1)(2k+1)}{6} + (k+1)^2 \\
    = & \frac{(k+1)[k(2k+1)+6(k+1)]}{6}  \\
    = & \frac{(k+1)(2k^2+7k+6)}{6}       \\
    = & \frac{(k+1)(2k^2+4k+3k+6)}{6}    \\
    = & \frac{(k+1)[2k(k+2)+3(k+2)]}{6}  \\
    = & \frac{(k+1)[(k+1)+1][2(k+1)+1]}{6}
    \end{IEEEeqnarray*}
    Then the formula holds for every $n$.
    \item If $n=1$, there is nothing to prove. If
    $n=k$ holds for the equation, then for $n=k+1$,
    \begin{IEEEeqnarray*}{lC}
      & [1+\dots+k+(k+1)]^2 \\
    = & (1+\dots+k)^2 + (k+1)^2 + 2(k+1)(1+\dots+k) \\
    = & 1^3+\dots+k^3 + (k+1)[(k+1)+2\frac{k(k+1)}{2}] \\
    = & 1^3+\dots+k^3 + (k+1)^3
    \end{IEEEeqnarray*}
    This finishes the proof for every $n$.
  \end{enumerate}
\end{solution}

\begin{pr} % 2.2
  Find a formula for
  \begin{enumerate}[label=(\roman*)]
    \item
    $\displaystyle\sum_{i=1}^n (2i-1) = 1+3+5+\dots+(2n-1)$.
    \item $\displaystyle\sum_{i=1}^n (2i-1)^2
    = 1^2 + 3^2 + 5^2 + \dots + (2n - 1)^2$.
  \end{enumerate}
  Hint: What do these expressions have to do with
  $1 + 2 + 3 + \dots + 2n$ and $1^2 + 2^2 + 3^2 + \dots
  + (2n)^2$?
\end{pr}

\begin{solution} % s2.2
  \begin{enumerate}[label=(\roman*)]
    \item Remind that $1+\dots+2n=n(2n+1)$ and
    that $2 + \dots + 2n = 2 \cdot \dfrac{n(n+1)}{2} = n(n+1)$.
    Hence,
    \begin{equation*}
      \sum_{i=1}^n (2i - 1) = n(2n+1) - n(n+1) = n^2
    \end{equation*}
    \item Using \autoref{2.1}\ref{2.1:i}, we easily
    derive that $\displaystyle
    \sum_{i=1}^{2n} i^2 = \dfrac{n(2n+1)(4n+1)}{3}$
    and $\displaystyle
    \sum_{i=1}^n (2i)^2 = \dfrac{2n(n+1)(2n+1)}{3}$.
    Therefore,
    \begin{equation*}
      \sum_{i=1}^n (2i - 1)^2 = \sum_{i=1}^{2n} i^2
      - \sum_{i=1}^n (2i)^2
      = \frac{n(4n^2 - 1)}{3}
    \end{equation*}
  \end{enumerate}
\end{solution}

\begin{pr} \label{2.3} % 2.3
  If $0 \leq k \leq n$, the ``binomial coefficient''
  $\displaystyle\binom{n}{k}$ is defined by
  $\displaystyle\binom{n}{k} = \dfrac{n!}{k!(n-k)!}
  = \dfrac{n(n-1)\cdots(n-k+1)}{k!}$, if $k\neq0,n$ \\
  $\displaystyle\binom{n}{0} = \binom{n}{n} = 1$.
  (This becomes a special case of the first formula
  if we define $0! = 1$.)
  \begin{enumerate}[label=(\alph*)]
    \item \label{2.3:a}
    Prove that
    \begin{equation*}
      \binom{n+1}{k} = \binom{n}{k-1} + \binom{n}{k}.
    \end{equation*}
    (The proof does not require an induction argument.)

    \medskip
    This relation gives rise to the following configuration,
    known as ``Pascal's triangle''---a number not on one of the
    sides is the sum of two numbers above it; the binomial
    coefficient $\displaystyle\binom{n}{k}$ is the
    $(k+1)$st number in the $(n+1)$st row.
    \par
    \begin{center} \label{PascalTriangle}
      \begin{tikzpicture}
        \foreach \n in {0,...,5}{
          \foreach \k in {0,...,\n}{
            \node at (\k - \n/2, -\n){$\binomialCoefficient{\n}{\k}$};
          }
        }
      \end{tikzpicture}
    \end{center}
    \item Notice that all numbers in Pascal's triangle are
    natural numbers. Use part \ref{2.3:a} to prove by
    induction that $\displaystyle\binom{n}{k}$ is always
    a natural number. (Your entire proof by induction will,
    in a sense, be summed up in a glance by Pascal's
    triangle.)
    \item Give another proof that $\displaystyle\binom{n}{k}$
    is a natural number by showing that
    $\displaystyle\binom{n}{k}$ is the number of sets of
    exactly $k$ integers each chosen from $1,\dots,n$.
    \item Prove the ``binomial theorem'': If $a$ and $b$
    are any numbers and $n$ is a natural number, then
    \begin{IEEEeqnarray*}{rCl}
      (a+b)^n & = & a^n + \binom{n}{1}a^{n-1}b
      + \binom{n}{2}a^{n-2}b^2+\cdots+\binom{n}{n-1}ab^{n-1}
      + b^n \\
              & = & \sum_{j=0}^n \binom{n}{j}a^{n-j}b^j.
    \end{IEEEeqnarray*}
    \item Prove that
    \begin{enumerate}[label=(\roman*)]
      \item \label{2.3:ei}
      $\displaystyle
      \sum_{j=0}^n \binom{n}{j}
      = \binom{n}{0} + \cdots + \binom{n}{n}
      = 2^n$.
      \item \label{2.3:eii}
      $\displaystyle
      \sum_{j=0}^n (-1)^j \binom{n}{j}
      = \binom{n}{0} - \binom{n}{1} + \cdots \pm \binom{n}{n}
      = 0$.
      \item $\displaystyle
      \sum_{l\text{ odd}} \binom{n}{l}
      = \binom{n}{1} + \binom{n}{3} + \cdots
      = 2^{n - 1}$.
      \item $\displaystyle
      \sum_{l\text{ even}} \binom{n}{l}
      = \binom{n}{0} + \binom{n}{2} + \cdots
      = 2^{n - 1}$.
    \end{enumerate}
  \end{enumerate}
\end{pr}

\begin{solution} % s2.3
  \begin{enumerate}[label=(\alph*)]
    \item Starting from the left-hand side,
    \begin{IEEEeqnarray*}{rCl}
      \binom{n + 1}{k} & = &
      \frac{n!(n - k + 1 + k)}{k!(n - k + 1)!} \\
                       & = &
      \frac{n!(n - k + 1)}{k!(n - k + 1)!}
    + \frac{n!k}{k!(n - k + 1)!}\\
                       & = &
      \frac{n!}{k!(n - k)!}
    + \frac{n!}{(k - 1)![n - (k - 1)]!} \\
                       & = &
      \binom{n}{k} + \binom{n}{k - 1}
    \end{IEEEeqnarray*}
    \item It is sufficient to prove that $\displaystyle
    \binom{n}{k}$ is a natural number for all
    $1 \leq k \leq (n - 1)$. If $n = 1$, then
    \begin{equation*}
      \binom{2}{1} = \binom{1}{0} + \binom{1}{1} = 2
    \end{equation*}
    Suppose that $\displaystyle\binom{n}{k}$ is natural
    number for any $n$ and $1 \leq k \leq n - 1$.
    Then for any $1 \leq k \leq n$, $\displaystyle
    \binom{n + 1}{k}$ is the sum of two natural numbers,
    and therefore it must be a natural number.
    \item It is sufficient to prove for the case
    $0 < k \leq n$.
    If $n=1$, the claim is trivial. Suppose that
    $\displaystyle\binom{n}{k}$ is the number of sets
    of $k$ integers each chosen from $1,\dots,n$; then
    $\displaystyle\binom{n + 1}{k}$ must include
    $\displaystyle\binom{n}{k}$ sets of $k$ integers
    \note{without} the newly added element and a number
    of sets of $k$ integers \note{with} the newly added
    element. The latter is exactly $\displaystyle
    \binom{n}{k - 1}$ and is a natural number by assumption.
    Thereby, $\displaystyle\binom{n+1}{k}$ must be
    a natural number.
    \item We prove by induction on $n$. If $n=1$, there
    is nothing to prove. Suppose the binomial theorem holds
    for $n$; then for $n+1$,
    \begin{IEEEeqnarray*}{rCl}
      (a+b)^n(a+b) & = &
      \sum_{j=0}^n \binom{n}{j} a^{n-j}b^j(a + b) \\
                   & = &
      \sum_{j=0}^n \binom{n}{j} a^{n+1-j}b^j
    + \sum_{j=0}^n \binom{n}{j} a^{n-j}b^{j+1}    \\
                   & = &
      a^{n + 1} + b^{n + 1}
    + \sum_{j=1}^n \binom{n}{j} a^{n+1-j}b^j      \\
                   & + &
      \sum_{j=1}^n \binom{n}{j-1} a^{n+1-j}b^j    \\
                   & = &
      \sum_{j=1}^n \binom{n+1}{j} a^{n+1-j}b^j
    + a^{n+1} + b^{n+1}                           \\
                   & = &
      \sum_{j=0}^{n+1} \binom{n+1}{j} a^{n+1-j}b^j
    \end{IEEEeqnarray*}
    which completes the proof.
    \item This part relies heavily on
    the binomial theorem from the above.
    \begin{enumerate}[label=(\roman*)]
      \item This is directly from the above: Applying
      the binomial theorem for $a=b=1$ yields the result.
      \item Let $a=1$ and $b=-1$ yield the result.
      \item Applying \ref{2.3:ei} $+$ \ref{2.3:eii},
      we derive that for $l$ even,
      \begin{equation*}
        \sum_{l\text{ even}} \binom{n}{l} = 2^{n - 1}
      \end{equation*}
      Thereby, $\displaystyle
      \sum_{l\text{ odd}} \binom{n}{l} = 2^n - 2^{n - 1}
      = 2^{n - 1}$.
      \item See the above.
    \end{enumerate}
    One thing to note: Both of the previous parts do not
    have a final term expressed in their sum due to the
    dependence of value $n$ (if $n$ is even or odd).
  \end{enumerate}
\end{solution}

\begin{pr} \label{2.4} % 2.4
  \begin{enumerate}[label=(\alph*)]
    \item \label{2.4:a}
    Prove that
    \begin{equation*}
      \sum_{k=0}^l \binom{n}{k} \binom{m}{l-k}
      = \binom{n+m}{l}.
    \end{equation*}
    Hint: Apply the binomial theorem to $(1+x)^n(1+x)^m$.
    \item \label{2.4:b}
    Prove that
    \begin{equation*}
      \sum_{k=0}^n \binom{n}{k}^2 = \binom{2n}{n}.
    \end{equation*}
  \end{enumerate}
\end{pr}

\begin{solution} % 2.4 solved
  \begin{enumerate}[label=(\alph*)]
    \item Remind that $(1+x)^n(1+x)^m = (1+x)^{n+m}$. Hence,
    \begin{equation*}
      \sum_{k=0}^n \binom{n}{k}x^k \cdot
      \sum_{j=0}^m \binom{m}{j}x^j
      = \sum_{l=0}^{n+m} \binom{n+m}{l}x^l
    \end{equation*}
    Observing that each term of $x^l$ is
    \begin{equation*}
      \sum_{k=0}^l \binom{n}{k}\binom{m}{l-k}
    \end{equation*}
    for every $k$ and $j$ such that $j = l - k$.
    \item From \ref{2.4:a}, let $m = l = n$ and observe
    that for all $0\leq k\leq n$,
    \begin{equation*}
      \binom{n}{k} = \binom{n}{n - k}
    \end{equation*}
    since $\dfrac{n!}{k!(n-k)!} = \dfrac{n!}{(n-k)!k!}$.
    Hence,
    $\displaystyle\sum_{k=0}^n \binom{n}{k}^2 = \binom{2n}{n}$.
  \end{enumerate}
\end{solution}

\begin{pr} \label{2.5} % 2.5
  \begin{enumerate}[label=(\alph*)]
    \item \label{2.5:a}
    Prove by induction on $n$ that
    \begin{equation*}
      1 + r + r^2 + \cdots + r^n = \frac{1-r^{n+1}}{1-r}
    \end{equation*}
    if $r\neq1$ (if $r=1$, evaluating the sum certainly
    presents no problem).
    \item \label{2.5:b}
    Derive this result by setting $S = 1 + r + \cdots + r^n$,
    multiplying this equation by $r$, and solving the
    two equations for $S$.
  \end{enumerate}
\end{pr}

\begin{solution} % 2.5 solved
  \begin{enumerate}[label=(\alph*)]
    \item If $n=1$, then the formula immediately holds. Suppose
    now that it holds for $n$, then for $n+1$,
    \begin{IEEEeqnarray*}{rCl}
      1 + r + \cdots + r^n + r^{n+1}
    & = & \frac{1 - r^{n+1}}{1-r} + r^{n+1} \\
    & = & \frac{1 - r^{n + 2}}{1 - r}
  \end{IEEEeqnarray*}
  which completes the proof.
    \item Let
    \begin{equation*}
      S = 1 + r + r^2 + \cdots + r^n
    \end{equation*}
    then
    \begin{equation*}
      rS = r + r^2 + r^3 + \cdots + r^{n+1}
    \end{equation*}
    Solving for $S$, we easily obtain
    \begin{equation*}
      S = \frac{1 - r^{n+1}}{1 - r}
    \end{equation*}
  \end{enumerate}
\end{solution}

\begin{pr} \label{2.6} % 2.6
  The formula for $1^2 + \cdots + n^2$ may be derived as
  follows. We begin with the formula
  \begin{equation*}
    (k+1)^3 - k^3 = 3k^2 + 3k + 1.
  \end{equation*}
  Writing this formula for $k=1,\dots,n$ and adding,
  we obtain

  \bigskip
  \begin{IEEEeqnarray*}{rCl}
    2^3 - 1^3 & = & 3 \cdot 1^2 + 3 \cdot 1 + 1 \\
    3^3 - 2^3 & = & 3 \cdot 2^2 + 3 \cdot 2 + 1 \\
    \vdots                                      \\
    (n + 1)^3 - n^3 & = & 3 \cdot n^2 + 3 \cdot n + 1 \\
    \hline                                            \\
    (n + 1)^3 - 1 & = & 3[1^2 + \cdots + n^2]
    + 3[1 + \cdots + n] + n.
  \end{IEEEeqnarray*}

  \bigskip
  Thus we can find
  $\displaystyle \sum_{k=1}^n k^2$ if we already know
  $\displaystyle \sum_{k=1}^n k$ (which could have been
  found in a similar way). Use this method to find
  \begin{enumerate}[label=(\roman*)]
    \item $1^3 + \cdots + n^3$.
    \item $1^4 + \cdots + n^4$.
    \item $\displaystyle
    \frac{1}{1\cdot2} + \frac{1}{2\cdot3} + \cdots
    + \frac{1}{n(n + 1)}$.
    \item $\displaystyle
    \frac{3}{1^2\cdot2^2} + \frac{5}{2^2\cdot3^2} + \cdots
    + \frac{2n + 1}{n^2(n + 1)^2}$.
  \end{enumerate}
\end{pr}

\begin{solution} % 2.6 solved
  \begin{enumerate}[label=(\roman*)]
    \item We easily derive that
    \begin{equation*}
      (k+1)^4 - k^4 = 4k^3 + 6k^2 + 4k + 1
    \end{equation*}
    Hence,
    \begin{IEEEeqnarray*}{rCl}
      2^4 - 1^4 &=& 4\cdot1^3 + 6\cdot1^2 + 4\cdot1 + 1 \\
      3^4 - 2^4 &=& 4\cdot2^3 + 6\cdot2^2 + 4\cdot2 + 1 \\
      \vdots                                            \\
      (n + 1)^4 - n^4 &=& 4\cdot n^3 + 6 \cdot n^2
      + 4 \cdot n + 1                                   \\
      \hline                                            \\
      (n + 1)^4 - 1 &=& 4[1^3 + 2^3 + \cdots + n^3]     \\
      & + & 6[1^2 + 2^2 + \cdots + n^2] + 4[1 + 2 + \cdots + n]
      + n
    \end{IEEEeqnarray*}
    It is easily derivable that
    \begin{equation*}
      1^3 + \cdots + n^3 = \frac{1}{4}n^2(n + 1)^2
    \end{equation*}
    \item The easiest way to calculate
    $(k + 1)^5 - k^5$ is to use the Pascal triangle from
    page \pageref{PascalTriangle}: We derive the result
    \begin{equation*}
      (k + 1)^5 - k^5 = 5k^4 + 10k^3 + 10k^2 + 5k + 1
    \end{equation*}
    A similar step from above shows that
    \begin{IEEEeqnarray*}{rCl}
      (n + 1)^5 - 1 & = & 5[1^4 + \cdots + n^4]
      + 10[1^3 + \cdots + n^3] \\
                      & + & 10[1^2 + \cdots + n^2]
      + 5[1 + \cdots + n] + n
    \end{IEEEeqnarray*}
    We derive from the available results,
    \begin{equation*}
      1^4 + 2^4 + \cdots + n^4 = \frac{1}{30}
      n(n+1)(2n+1)(3n^2 + 3n - 1)
    \end{equation*}
    \item Observe that
    \begin{equation*}
      \frac{1}{k} - \frac{1}{k + 1} = \frac{1}{k(k + 1)}
    \end{equation*}
    Henceforth,
    \begin{IEEEeqnarray*}{rCl}
      1 - \frac{1}{2} &=& \frac{1}{1\cdot2} \\
      \frac{1}{2} - \frac{1}{3} &=& \frac{1}{2\cdot3} \\
      \vdots                                          \\
      \frac{1}{n} - \frac{1}{n + 1}
      &=& \frac{1}{n\cdot(n+1)}                       \\
      \hline                                          \\
      1 - \frac{1}{n + 1} & = &
      \frac{1}{1\cdot2} + \frac{1}{2\cdot3} + \cdots
      + \frac{1}{n(n + 1)}                            \\
      \frac{1}{1\cdot2} + \frac{1}{2\cdot3} + \cdots
      + \frac{1}{n(n + 1)}& = & \frac{n}{n + 1}
    \end{IEEEeqnarray*}
    \item See that
    \begin{equation*}
      \frac{1}{k^2} - \frac{1}{(k+1)^2}
      = \frac{2k + 1}{k^2(k + 1)^2}
    \end{equation*}
    Henceforth,
    \begin{IEEEeqnarray*}{rCl}
      1 - \frac{1}{2^2} &=& \frac{3}{1^2\cdot2^2} \\
      \frac{1}{2^2} - \frac{1}{3^2} &=& \frac{5}{2^2\cdot3^2} \\
      \vdots \\
      \frac{1}{n^2} - \frac{1}{(n+1)^2} &=&
      \frac{2n + 1}{n^2(n + 1)^2}                  \\
      \hline                                       \\
      \frac{3}{1^2\cdot2^2} + \frac{5}{2^2\cdot3^2}
      + \cdots + \frac{2n + 1}{n^2(n + 1)^2}
      & = & \frac{n(n+2)}{(n+1)^2}
    \end{IEEEeqnarray*}
  \end{enumerate}
\end{solution}
